src/tls/PSK.fst
@@ -24,14 +24,18 @@ module HH = FStar.HyperHeap
 //  - for tickets, the encrypted serialized state is the PSK identifier
 //  - we store in the table the PSK context and compromise status
 
-type psk_context = {
+type pskInfo = {
   time_created: int;
   allow_early_data: bool;      // New draft 13 flag
   allow_dhe_resumption: bool;  // New draft 13 flag
   allow_psk_resumption: bool;  // New draft 13 flag
   early_ae: aeadAlg;
   early_hash: CoreCrypto.hash_alg;
+  identities: bytes * bytes;
 }
+
+let pskInfo_hash pi = pi.early_hash
+let pskInfo_ae pi = pi.early_ae
 
 type psk_identifier = identifier:bytes{length identifier < 65536}
 
@@ -41,14 +45,14 @@ let app_psk (i:psk_identifier) =
   b:bytes{exists i.{:pattern index b i} index b i <> 0z}
 
 type app_psk_entry (i:psk_identifier) =
-  (app_psk i) * ctx:psk_context * leaked:(rref tls_tables_region bool)
+  (app_psk i) * pskInfo * leaked:(rref tls_tables_region bool)
 
 
 // ADL: not sure why b2t is required there
 let app_psk_injective (m:MM.map' psk_identifier app_psk_entry) =
   forall i1 i2.{:pattern (MM.sel m i1); (MM.sel m i2)}
-      b2t (equalBytes i1 i2) <==> (match MM.sel m i1, MM.sel m i2 with
-                  | Some (psk1, _, _), Some (psk2, _, _) -> b2t (equalBytes psk1 psk2)
+      Seq.equal i1 i2 <==> (match MM.sel m i1, MM.sel m i2 with
+                  | Some (psk1, _, _), Some (psk2, _, _) -> Seq.equal psk1 psk2
                   | _ -> True)
 
 private let app_psk_table : MM.t tls_tables_region psk_identifier app_psk_entry app_psk_injective =
@@ -57,44 +61,28 @@ private let app_psk_table : MM.t tls_tables_region psk_identifier app_psk_entry 
 let fresh_pskid i h =
   MM.sel (MR.m_sel h app_psk_table) i = None
 
-// Is the identifier i currently registered as an application PSK?
-//val registered_app_psk: i:psk_identifier -> h:HH.t -> GTot Type
 let registered_app_psk (i:psk_identifier) (h:HH.t) =
   b2t (is_Some (MM.sel (MR.m_sel h app_psk_table) i))
 
-let app_psk_hash (i:psk_identifier) (hash:CoreCrypto.hash_alg) (h:HH.t) =
+let valid_app_psk (ctx:pskInfo) (i:psk_identifier) (h:HH.t) =
   match MM.sel (MR.m_sel h app_psk_table) i with
-  | Some (_, c, _) -> b2t (c.early_hash = hash)
+  | Some (_, c, _) -> b2t (c = ctx)
   | _ -> False
-
-//  b2t (is_Some (MM.sel (MR.m_sel h app_psk_table) i))
-//  /\ let Some () = 
 
 type ex_app_psk = i:psk_identifier{MR.witnessed (registered_app_psk i)}
 
 let fresh_psk psk (h:HH.t) =
   forall i. match MM.sel (MR.m_sel h app_psk_table) i with
-       | Some (psk', _, _) -> ~ (b2t (equalBytes psk psk'))
+       | Some (psk', _, _) -> ~ (Seq.equal psk psk')
        | None -> True
 
-//private val app_psk_context: i:psk_identifier -> ST psk_context
-//  (requires (fun h -> registered_app_psk i h))
-//  (ensures (fun h0 r h1 -> h0=h1))
-let app_psk_context (i:ex_app_psk) =
-  let (_, c, _) = Some.v (MM.lookup app_psk_table i) in c
-
-//private val app_psk_value: i:psk_identifier -> ST (app_psk i)
-//  (requires (fun h -> registered_app_psk i h))
-//  (ensures (fun h0 r h1 -> h0=h1))
-let app_psk_value (i:ex_app_psk) =
+let app_psk_value (i:ex_app_psk) : St (app_psk i) =
   let (psk, _, _) = Some.v (MM.lookup app_psk_table i) in psk
 
 // Attacker interface
-// TODO not monotonic, we are in a world of pain
-
-let leak i:ex_app_psk =
-  let (v, _, l) = Some.v (MM.lookup app_psk_table i) in
-  l := true; v
+//let leak i:ex_app_psk =
+//  let (v, _, l) = Some.v (MM.lookup app_psk_table i) in
+//  l := true; v
 
 // Generates a fresh PSK identity
 val fresh_psk_id: unit -> ST psk_identifier
@@ -110,7 +98,7 @@ let rec fresh_psk_id () =
 // "Application PSK" generator (enforces empty session context)
 // Usual caveat of random producing pairwise distinct keys (TODO)
 
-let gen_psk (i:psk_identifier) (ctx:psk_context)
+let gen_psk (i:psk_identifier) (ctx:pskInfo)
   : ST unit
   (requires (fun h -> fresh_pskid i h))
   (ensures (fun h0 r h1 ->
